coq/SoundSequal.v
@@ -1,0 +1,515 @@
+
+Require Import Coq.Lists.List.
+Import ListNotations.
+
+Require Import Tactics.
+Require Import Axioms.
+Require Import Sigma.
+Require Import Equality.
+Require Import Sequence.
+Require Import Relation.
+Require Import Ordinal.
+Require Import Syntax.
+Require Import SimpSub.
+Require Import Dynamic.
+Require Import Ofe.
+Require Import Uniform.
+Require Import Intensional.
+Require Import Candidate.
+Require Import System.
+Require Import Semantics.
+Require Import SemanticsKnot.
+Require Import Judgement.
+Require Import Hygiene.
+Require Import ProperClosed.
+Require Import ProperFun.
+Require Import Shut.
+
+Require Import SemanticsSimple.
+Require Import ProperLevel.
+Require Import Equivalence.
+Require Import Subsumption.
+Require Import ProperEquiv.
+Require Import Truncate.
+Require Import ProperDownward.
+Require Import Equivalences.
+
+
+
+Local Ltac prove_hygiene :=
+  repeat (apply hygiene_auto; cbn; repeat2 split; auto);
+  eauto using hygiene_weaken, clo_min, hygiene_shift', hygiene_subst1, subst_closub;
+  try (apply hygiene_var; cbn; auto; done).
+
+
+
+Lemma sound_sequal_formation :
+  forall G m n,
+    pseq G (deqtype (sequal m m) (sequal n n)).
+Proof.
+intros G m n.
+revert G.
+refine (seq_pseq 2 [] m [] n 0 _ _); cbn.
+intros G Hclm Hcln.
+rewrite -> seq_eqtype.
+intros i s s' Hs.
+so (pwctx_impl_closub _#4 Hs) as (Hcls & Hcls').
+so (subst_closub _#4 Hcls Hclm) as Hclm'.
+so (subst_closub _#4 Hcls' Hclm) as Hclm''.
+so (subst_closub _#4 Hcls Hcln) as Hcln'.
+so (subst_closub _#4 Hcls' Hcln) as Hcln''.
+exists (iubase (unit_urel stop i)); auto using interp_eval_refl, interp_sequal.
+simpsub.
+do2 3 split; auto.
+  {
+  apply interp_eval_refl.
+  apply interp_sequal; auto.
+  apply equiv_refl.
+  }
+
+  {
+  apply interp_eval_refl.
+  apply interp_sequal; auto.
+  apply equiv_refl.
+  }
+  {
+  apply interp_eval_refl.
+  apply interp_sequal; auto.
+  apply equiv_refl.
+  }
+
+  {
+  apply interp_eval_refl.
+  apply interp_sequal; auto.
+  apply equiv_refl.
+  }
+Qed.
+
+
+
+Lemma sound_sequal_intro :
+  forall G m,
+    pseq G (deq triv triv (sequal m m)).
+Proof.
+intros G m.
+revert G.
+refine (seq_pseq 1 [] m 0 _ _); cbn.
+intros G Hclm.
+rewrite -> seq_deq.
+intros i s s' Hs.
+so (pwctx_impl_closub _#4 Hs) as (Hcls & Hcls').
+so (subst_closub _#4 Hcls Hclm) as Hclm'.
+so (subst_closub _#4 Hcls' Hclm) as Hclm''.
+exists (iubase (unit_urel stop i)); auto using interp_eval_refl, interp_sequal.
+simpsub.
+rewrite -> den_iubase.
+assert (rel (unit_urel stop i) i triv triv) as Htriv.
+  {
+  do2 5 split; auto using star_refl.
+    {
+    apply hygiene_auto; cbn; auto.
+    }
+
+    {
+    apply hygiene_auto; cbn; auto.
+    }
+  }
+do2 4 split; auto.
+  {
+  apply interp_eval_refl.
+  apply interp_sequal; auto.
+  apply equiv_refl.
+  }
+
+  {
+  apply interp_eval_refl.
+  apply interp_sequal; auto.
+  apply equiv_refl.
+  }
+Qed.
+
+
+
+Lemma sound_sequal_eta :
+  forall G m n p,
+    pseq G (deq p p (sequal m n))
+    -> pseq G (deq p triv (sequal m n)).
+Proof.
+intros G m n p.
+revert G.
+refine (seq_pseq 0 1 [] _ _ _); cbn.
+intros G Hseq.
+rewrite -> seq_deq in Hseq |- *.
+intros i s s' Hs.
+so (Hseq _#3 Hs) as (R & Hequall & Hequalr & Htrue & _).
+simpsubin Hequall.
+invert (basic_value_inv _#6 value_sequal Hequall).
+intros _ _ _ Heq.
+exists R.
+do2 4 split; auto.
+  {
+  simpsub.
+  subst R.
+  do2 5 split; auto using star_refl.
+    {
+    apply hygiene_auto; cbn; auto.
+    }
+
+    {
+    apply hygiene_auto; cbn; auto.
+    }
+  }
+
+  {
+  simpsub.
+  subst R.
+  destruct Htrue as (_ & _ & Hclsp & Hclsp' & Hsteps & _).
+  do2 5 split; auto using star_refl.
+    {
+    apply hygiene_auto; cbn; auto.
+    }
+  }
+Qed.
+
+
+Lemma sound_sequal_eta_hyp :
+  forall G1 G2 p q m n b,
+    pseq (substctx (dot triv id) G2 ++ G1) (deq m n (subst (under (length G2) (dot triv id)) b))
+    -> pseq (G2 ++ hyp_tm (sequal p q) :: G1) (deq (subst (under (length G2) sh1) m) (subst (under (length G2) sh1) n) b).
+Proof.
+intros G1 G2 p q m n b Hseq.
+eapply sound_property_eta_hyp; eauto.
+intros s pg z i R H.
+simpsubin H.
+invert (basic_value_inv _#6 value_sequal H).
+intros _ _ _ _ <-.
+do 3 eexists; reflexivity.
+Qed.
+
+
+Lemma sound_syntactic_substitution :
+  forall G1 G2 a m n n' b,
+    pseq 
+      (substctx (dot (var 0) (dot (subst (sh 2) m) (sh 2))) G2 ++ hyp_tm (sequal (var 0) (subst sh1 m)) :: hyp_tm a :: G1) 
+      (deq n n' (subst (under (length G2) (dot (var 0) (dot (subst (sh 2) m) (sh 2)))) b))
+    -> pseq 
+         (G2 ++ hyp_tm (sequal (var 0) (subst sh1 m)) :: hyp_tm a :: G1)
+         (deq n n' b).
+Proof.
+intros G1 G2 a m n n' b.
+revert G1.
+refine (seq_pseq_hyp 2 [] m (G2 ++ [hyp_tm (sequal (var 0) (subst sh1 m)); hyp_tm a]) b 1 _ [_; _] _ _ [_; _] _ _); cbn.
+intros G1 Hclm Hclb Hseq _.
+assert (subsume 
+          (hyp_tm (sequal (var 0) (subst sh1 m)) :: hyp_tm a :: G1)
+          (hyp_tm (sequal (var 0) (subst sh1 m)) :: hyp_tm a :: G1)
+          id
+          (dot (var 0) (dot (subst (sh 2) m) (sh 2)))) as Hsubsume.
+  {
+  clear b Hclb Hseq n n'.
+  do2 2 split.
+    {
+    intro j.
+    cbn.
+    split.
+      {
+      intro H.
+      destruct j as [|[ | j]].
+        {
+        simpsub.
+        apply hygiene_var; auto.
+        }
+
+        {
+        simpsub.
+        apply hygiene_shift'; auto.
+        }
+
+        {
+        simpsub.
+        apply hygiene_var; auto.
+        }
+      }
+
+      {
+      intro H.
+      destruct j as [|[| j]].
+        {
+        cbn.
+        auto.
+        }
+
+        {
+        cbn; auto.
+        }
+
+        {
+        cbn.
+        simpsubin H.
+        invert H.
+        cbn.
+        auto.
+        }
+      }
+    }
+
+    {
+    intro j.
+    cbn.
+    split.
+      {
+      intro H.
+      simpsub.
+      apply hygiene_var.
+      auto.
+      }
+
+      {
+      intro H.
+      simpsubin H.
+      cbn in H.
+      invert H; auto.
+      }
+    }
+    
+    {
+    intros i ss ss' Hss.
+    invert Hss.
+    intros n n' ss1 ss1' Hss1 Hn _ _ <- <-.
+    invertc Hss1.
+    intros p p' s s' Hs Hp Hleft Hright <- <-.
+    simpsubin Hn.
+    invertc Hn.
+    intros R Hl Hr _.
+    invert (basic_value_inv _#6 value_sequal Hl).
+    intros _ _ Hequiv _.
+    invert (basic_value_inv _#6 value_sequal Hr).
+    intros _ _ Hequiv' _.
+    clear R Hl Hr.
+    do2 4 split; auto.
+      {
+      simpsub.
+      apply equivsub_dot; auto using equiv_refl.
+      apply equivsub_dot; auto using equivsub_refl.
+      apply equiv_symm; auto.
+      }
+
+      {
+      simpsub.
+      apply equivsub_dot; auto using equiv_refl.
+      apply equivsub_dot; auto using equivsub_refl.
+      apply equiv_symm; auto.
+      }
+
+      {
+      intros j b t Hj Htt.
+      simpsubin Htt.
+      rewrite -> !qpromote_cons in Htt |- *.
+      rewrite -> !qpromote_hyp_tm in Htt |- *.
+      invert Htt.
+      intros n'' tt1 Htt1 Hn'' <-.
+      invertc Htt1.
+      intros p'' t Ht Hp'' <-.
+      simpsub.
+      simpsubin Hn''.
+      invert Hn''.
+      intros R _ HR _.
+      invert (basic_value_inv _#6 value_sequal HR).
+      intros Hclp'' Hcltm Hequivp''_tm _.
+      clear R HR.
+      simpsubin Hp''.
+      apply seqctx_cons.
+        {
+        apply seqctx_cons; auto.
+        simpsub.
+        invert Hp''.
+        intros R Hl Hr H.
+        apply (seqhyp_tm _#5 R); auto.
+        eapply urel_equiv_2; eauto.
+        }
+
+        {
+        simpsub.
+        eapply seqhyp_equivh_2; eauto.
+          {
+          apply equivh_tm.
+          apply equiv_sequal; auto using equiv_refl.
+          }
+
+          {
+          apply hygieneh_tm.
+          apply hygiene_auto; cbn; auto.
+          }
+        }
+      }
+
+      {
+      intros j b t Hj Htt.
+      simpsubin Htt.
+      rewrite -> !qpromote_cons in Htt |- *.
+      rewrite -> !qpromote_hyp_tm in Htt |- *.
+      invert Htt.
+      intros n'' tt1 Htt1 Hn'' <-.
+      invertc Htt1.
+      intros p'' t Ht Hp'' <-.
+      simpsub.
+      simpsubin Hn''.
+      invert Hn''.
+      intros R HR _ _.
+      invert (basic_value_inv _#6 value_sequal HR).
+      intros Hclp'' Hcltm Hequivp''_tm _.
+      clear R HR.
+      simpsubin Hp''.
+      apply seqctx_cons.
+        {
+        apply seqctx_cons; auto.
+        simpsub.
+        invert Hp''.
+        intros R Hl Hr H.
+        apply (seqhyp_tm _#5 R); auto.
+        eapply urel_equiv_1; eauto.
+        }
+
+        {
+        simpsub.
+        eapply seqhyp_equivh_1; eauto.
+          {
+          apply equivh_tm.
+          apply equiv_sequal; auto using equiv_refl.
+          }
+
+          {
+          apply hygieneh_tm.
+          apply hygiene_auto; cbn; auto.
+          }
+        }
+      }
+    }
+  }
+rewrite -> seq_deq in Hseq |- *.
+intros i s s' Hs.
+so (subsume_under _ _ G2 _ _ Hsubsume anderr _#3 Hs) as (Hs' & Heqs & Heqs' & _).
+rewrite <- compose_assoc in Heqs, Heqs'.
+rewrite <- compose_under in Heqs, Heqs'.
+so (Hseq _#3 Hs') as (B & Hbl & Hbr & Hnl & Hnr & Hnlr).
+exists B.
+simpsubin Hbl.
+simpsubin Hbr.
+rewrite <- compose_assoc in Hbl, Hbr.
+rewrite <- compose_under in Hbl, Hbr.
+so (pwctx_impl_closub _#4 Hs) as (Hcls & Hcls').
+rewrite <- app_assoc in Hclb.
+cbn [List.app] in Hclb.
+rewrite -> subst_compose in Hnl.
+rewrite -> subst_compose in Hnl.
+rewrite -> subst_compose in Hnr.
+rewrite -> subst_compose in Hnr.
+rewrite -> subst_compose in Hnlr.
+rewrite -> subst_compose in Hnlr.
+rewrite -> !(subst_eqsub _#4 (eqsub_under_id _ _)) in Hnl.
+rewrite -> !(subst_eqsub _#4 (eqsub_under_id _ _)) in Hnr.
+rewrite -> !(subst_eqsub _#4 (eqsub_under_id _ _)) in Hnlr.
+simpsubin Hnl.
+simpsubin Hnr.
+simpsubin Hnlr.
+do2 4 split; auto.
+  {
+  eapply basic_equiv; eauto.
+    {
+    eapply subst_closub; eauto.
+    }
+
+    {
+    apply equiv_funct; auto using equiv_refl.
+    }
+  }
+
+  {
+  eapply basic_equiv; eauto.
+    {
+    eapply subst_closub; eauto.
+    }
+
+    {
+    apply equiv_funct; auto using equiv_refl.
+    }
+  }
+Qed.
+
+
+
+Lemma sound_sequal_symm :
+  forall G m n,
+    pseq G (deq triv triv (sequal m n))
+    -> pseq G (deq triv triv (sequal n m)).
+Proof.
+intros G m n.
+revert G.
+refine (seq_pseq 0 1 [] _ _ _); cbn.
+intros G Hseq.
+rewrite -> seq_deq in Hseq |- *.
+intros i s s' Hs.
+so (Hseq _#3 Hs) as (R & Hl & Hr & Hinh & _).
+simpsubin Hl.
+simpsubin Hr.
+invert (basic_value_inv _#6 value_sequal Hl).
+intros Hclsm Hclsn Hequiv <-.
+invert (basic_value_inv _#6 value_sequal Hr).
+intros Hclsm' Hclsn' Hequiv'.
+exists (iubase (unit_urel stop i)).
+do2 4 split; auto.
+  {
+  apply interp_eval_refl.
+  simpsub.
+  apply interp_sequal; auto using equiv_symm.
+  }
+
+  {
+  apply interp_eval_refl.
+  simpsub.
+  apply interp_sequal; auto using equiv_symm.
+  }
+Qed.
+            
+
+
+Lemma sound_sequal_trans :
+  forall G m n p,
+    pseq G (deq triv triv (sequal m n))
+    -> pseq G (deq triv triv (sequal n p))
+    -> pseq G (deq triv triv (sequal m p)).
+Proof.
+intros G m n p.
+revert G.
+refine (seq_pseq 0 2 [] _ [] _ _ _); cbn.
+intros G Hmn Hnp.
+rewrite -> seq_deq in Hmn, Hnp |- *.
+intros i s s' Hs.
+so (Hmn _#3 Hs) as (R & Hl1 & Hr1 & Hinh & _).
+so (Hnp _#3 Hs) as (R' & Hl2 & Hr2 & _).
+simpsubin Hl1.
+simpsubin Hr1.
+simpsubin Hl2.
+simpsubin Hr2.
+invert (basic_value_inv _#6 value_sequal Hl1).
+intros Hclsm _ Hequivmn <-.
+invert (basic_value_inv _#6 value_sequal Hr1).
+intros Hclsm' _ Hequivmn'.
+invert (basic_value_inv _#6 value_sequal Hl2).
+intros _ Hclsp Hequivnp <-.
+invert (basic_value_inv _#6 value_sequal Hr2).
+intros _ Hclsp' Hequivnp'.
+exists (iubase (unit_urel stop i)).
+do2 4 split; auto.
+  {
+  apply interp_eval_refl.
+  simpsub.
+  apply interp_sequal; eauto using equiv_trans.
+  }
+
+  {
+  apply interp_eval_refl.
+  simpsub.
+  apply interp_sequal; eauto using equiv_trans.
+  }
+Qed.
